@prefix : <https://wikipunk.net/ssvc/> .
@prefix dcterms: <http://purl.org/dc/terms/> .
@prefix owl: <http://www.w3.org/2002/07/owl#> .
@prefix rdf: <http://www.w3.org/1999/02/22-rdf-syntax-ns#> .
@prefix rdfs: <http://www.w3.org/2000/01/rdf-schema#> .
@prefix xsd: <http://www.w3.org/2001/XMLSchema#> .
@prefix spdx: <http://spdx.org/rdf/terms#> .
@prefix d3f: <http://d3fend.mitre.org/ontologies/d3fend.owl#>
@prefix prov: <http://www.w3.org/ns/prov#> .
@prefix skos: <http://www.w3.org/2004/02/skos/core#> .
@prefix jsonschema: <https://www.w3.org/2019/wot/json-schema#> .
@prefix stix: <http://docs.oasis-open.org/cti/ns/stix#> .
@prefix tac: <http://docs.oasis-open.org/cti/ns/tac#> .

: a owl:Ontology ;
  owl:versionInfo "2.03" ;
  owl:imports (
    <http://d3fend.mitre.org/ontologies/d3fend.owl>
    <http://docs.oasis-open.org/cti/ns/stix>
    <http://docs.oasis-open.org/cti/ns/tac>
    ) ;
  prov:wasDerivedFrom (
    <https://github.com/CERTCC/SSVC/raw/main/data/schema/SSVC_Computed_v2.03.schema.json>
    <https://github.com/CERTCC/SSVC/raw/main/data/schema/SSVC_Provision_v2.03.schema.json>
    ) ;
  rdfs:label "Stakeholder-Specific Vulnerability Categorization Ontology" ;
  rdfs:comment  "The SSVC Ontology is a formal representation of the concepts, relationships, and structure of the Stakeholder-Specific Vulnerability Categorization (SSVC) framework. It provides a standardized model to represent decision trees, decision points, options, and computed scores for the prioritization of vulnerability remediation efforts. The ontology enables consistent communication, sharing, and analysis of SSVC scores and related information among different stakeholders, including vulnerability analysts, software developers, and security researchers." ;
  rdfs:seeAlso <https://resources.sei.cmu.edu/asset_files/WhitePaper/2021_019_001_653461.pdf> .

:DecisionTree a owl:Class ;
  rdfs:label "Decision Tree" ;
  rdfs:comment "A decision tree used in computing SSVC scores for a vulnerability." ;
  skos:definition "A DecisionTree represents a structured framework used within the SSVC process for vulnerability prioritization. The tree is made up of nodes, which correspond to different decision points based on various aspects or properties relevant to assessing vulnerabilities. Branches in the tree represent the possible options for each decision point." .

:DecisionPoint a owl:Class ;
  rdfs:label "Decision Point" ;
  rdfs:comment "A node in the decision tree, including the root node, with a label and two or more options" .

:Option a owl:Class ;
  rdfs:label "Option" ;
  rdfs:comment "An option within a decision point" .

:DecisionType a owl:Class ;
  rdfs:label "Decision Type" ;
  rdfs:comment "A decision type, which can be simple, complex, or final" ;
  owl:oneOf (
    :Simple
    :Complex
    :Final
    ) .

:Simple a :DecisionType ;
  rdfs:label "Simple Decision Type" ;
  rdfs:comment "A decision type that without children." .

:Complex a :DecisionType ;
  rdfs:label "Complex Decision Type" ;
  rdfs:comment "A decision type with children." .

:Final a :DecisionType ;
  rdfs:label "The last node on the decision tree." .

:Decision a owl:Class ;
  rdfs:label "Vulnerability Decision" ;
  rdfs:comment "A decision made when a vulnerability is discovered, determining the level of action required." .

:Color a owl:Class ;
  rdfs:label "Color" ;
  rdfs:comment "A color used to represent a decision" .

:Track a :Decision ;
  rdfs:label "Track" ;
  rdfs:comment "The vulnerability does not require action at this time. The organization would continue to track the vulnerability and reassess it if new information becomes available. CISA recommends remediating Track vulnerabilities within standard update guidelines." ;
  :hasColor "green" .

:TrackStar a :Decision ;
  rdfs:label "Track*" ;
  rdfs:comment "The vulnerability contains specific characteristics that may require closer monitoring for changes. CISA recommends remdiating Track* vulnerabilities within standard update guidelines." ;
  :hasColor "yellow" .

:Attend a :Decision ;
  rdfs:label "Attend" ;
  rdfs:comment "The vulnerability requires attention from the organization's internal, supervisory-level individuals. Necessary actions may include requesting assistance or information about the vulnerability and may involve publishing a notification, either internally and/or externally, about the vulnerability. CISA recommends remediating Attend vulnerabilities sooner than standard update timelines." ;
  :hasColor "orange" .

:Act a :Decision ;
  rdfs:label "Act" ;
  rdfs:comment "The vulnerability requires attention from the organization's internal, supervisory-level and leadership-level individuals. Necessary actions include requesting assistance or information about the vulnerability, as well as publishing a notification either internally and/or externally. Typically, internal groups would meet to determine the overall response and then execute agreed upon actions. CISA recommends remediating Act vulnerabilities as soon as possible." ;
  :hasColor "red" .

:hasDecision a owl:ObjectProperty ;
  rdfs:label "Has Vulnerability Decision" ;
  rdfs:comment "Relates a vulnerability to its decision" ;
  rdfs:domain d3f:Vulnerability ;
  rdfs:range :Decision .

:ComputedScore a owl:Class ;
  rdfs:label "Computed Score" ;
  rdfs:comment "A computed SSVC score representing the path in the decision tree" .

:hasDecisionPoint a owl:ObjectProperty ;
  rdfs:label "Has Decision Point" ;
  rdfs:comment "Relates a decision tree to its decision points" ;
  rdfs:domain :DecisionTree ;
  rdfs:range :DecisionPoint .

:hasOption a owl:ObjectProperty ;
  rdfs:label "Has Option" ;
  rdfs:comment "Relates a decision point to its options" ;
  rdfs:domain :DecisionPoint ;
  rdfs:range :Option .

:hasDecisionType a owl:ObjectProperty ;
  rdfs:label "Has Decision Type" ;
  rdfs:comment "Relates a decision point to its decision type" ;
  rdfs:domain :DecisionPoint ;
  rdfs:range :DecisionType .

:hasKey a owl:DatatypeProperty ;
  rdfs:label "Key" ;
  rdfs:comment "An optional short key that identifies a decision point or option in the SSVC score vector form" ;
  rdfs:domain :Decision ;
  rdfs:range xsd:string .

:hasColor a owl:DatatypeProperty ;
  rdfs:label "Color" ;
  rdfs:comment "An optional color to represent the final edge node or final recommended action provided by the SSVC tree" ;
  rdfs:range :DecisionPoint ;
  rdfs:range xsd:string .

:hasChild a owl:ObjectProperty ;
  rdfs:label "Has Child" ;
  rdfs:comment "Relates a decision point to its child decision points" ;
  rdfs:domain :DecisionPoint ;
  rdfs:range :DecisionPoint .

:hasParent a owl:ObjectProperty ;
  rdfs:label "Has Parent" ;
  rdfs:comment "Relates a decision point to its parent decision point" ;
  rdfs:domain :DecisionPoint ;
  rdfs:range :DecisionPoint .

:hasComputedScore a owl:DatatypeProperty ;
  rdfs:label "Has Computed Score" ;
  rdfs:comment "A short vector representation of an SSVC computed decision score" ;
  rdfs:domain :ComputedScore ;
  rdfs:range xsd:string .

:hasTimestamp a owl:DatatypeProperty ;
  rdfs:label "Has Timestamp" ;
  rdfs:comment "Date and time in ISO format (ISO 8601)" ;
  rdfs:domain :ComputedScore ;
  rdfs:range xsd:dateTime .

:hasRole a owl:DatatypeProperty ;
  rdfs:label "Has Role" ;
  rdfs:comment "Roles defined in the SSVC spec and optional in the SSVC provision schema" ;
  rdfs:domain :ComputedScore ;
  rdfs:range prov:Role .

:hasVersion a owl:DatatypeProperty ;
  rdfs:label "Has Version" ;
  rdfs:comment "Version of the SSVC that was used in this decision, in semver format" ;
  rdfs:domain :ComputedScore ;
  rdfs:range xsd:string .

:hasDecisionTree a owl:ObjectProperty ;
  rdfs:label "Has Decision Tree" ;
  rdfs:comment "The full decision tree that was used for this SSVC computed score" ;
  rdfs:domain :ComputedScore ;
  rdfs:range :DecisionTree .

:hasVulnerability a owl:DatatypeProperty ;
  rdfs:label "ID" ;
  rdfs:comment "Identifier for a vulnerability (CVE, CERT/CC VU#, OSV id, Bugtraq, etc.)" ;
  rdfs:domain :ComputedScore ;
  rdfs:range d3f:Vulnerability .

:hasDecisionTreeURL a owl:DatatypeProperty ;
  rdfs:label "Decision Tree URL" ;
  rdfs:comment "A URL that points to the decision tree used to make this computed decision" ;
  rdfs:domain :ComputedScore ;
  rdfs:range xsd:anyURI .

:hasSchema a owl:DatatypeProperty ;
  rdfs:label "Has Schema" ;
  rdfs:comment "A URL that points to the schema used for the decision tree to make this computed decision" ;
  rdfs:domain :ComputedScore ;
  rdfs:range xsd:anyURI .

:hasOptionPattern a owl:ObjectProperty ;
  rdfs:label "Has Option Pattern" ;
  rdfs:comment "Relates an option to the option patterns within it" ;
  rdfs:domain :Option ;
  rdfs:range xsd:string .

:Exploitation a :DecisionPoint ;
  rdfs:label "Exploitation" ;
  rdfs:comment "A decision point representing the current state of exploitation of a vulnerability, focusing on the present situation rather than predicting future exploitation." ;
  :hasOption :ExploitationNone, :ExploitationPoC, :ExploitationActive .

:ExploitationNone a :Option ;
  rdfs:label "None" ;
  rdfs:comment "There is no evidence of active exploitation and no public proof of concept (PoC) of how to exploit the vulnerability." .

:ExploitationPoC a :Option ;
  rdfs:label "PoC (Proof of Concept)" ;
  rdfs:comment "One of the following cases is true: (1) exploit code is sold or traded on underground or restricted fora; (2) a typical public PoC in places such as Metasploit or ExploitDB; or (3) the vulnerability has a well-known method of exploitation." .

:ExploitationActive a :Option ;
  rdfs:label "Active" ;
  rdfs:comment "Shared, observable, reliable evidence that the exploit is being used in the wild by real attackers; there is credible public reporting." .

:TechnicalImpact a :DecisionPoint ;
  rdfs:label "Technical Impact" ;
  rdfs:comment "A decision point representing the extent to which exploiting a vulnerability affects the control or information exposure of the software containing the vulnerability." ;
  :hasOption :TechnicalImpactPartial, :TechnicalImpactTotal .

:TechnicalImpactPartial a :Option ;
  rdfs:label "Partial" ;
  rdfs:comment "The exploit gives the adversary limited control over, or information exposure about, the behavior of the software that contains the vulnerability. Or the exploit gives the adversary an importantly low stochastic opportunity for total control. Denial of service is a form of limited control over the behavior of the vulnerable component." .

:TechnicalImpactTotal a :Option ;
  rdfs:label "Total" ;
  rdfs:comment "The exploit gives the adversary total control over the behavior of the software, or it gives total disclosure of all information on the system that contains the vulnerability." .

:Utility a :DecisionPoint ;
  rdfs:label "Utility" ;
  rdfs:comment "A decision point representing the usefulness of the exploit to an adversary, based on the assumption that they can exploit the vulnerability. Utility is independent from the state of Exploitation and is a combination of the value density of vulnerable components and whether potential exploitation is automatable." ;
  :hasOption :UtilityLaborious, :UtilityEfficient, :UtilitySuperEffective .

:UtilityLaborious a :Option ;
  rdfs:label "Laborious" ;
  rdfs:comment "No to automatable and diffuse value." .

:UtilityEfficient a :Option ;
  rdfs:label "Efficient" ;
  rdfs:comment "{Yes to automatable and diffuse value} OR {No to automatable and concentrated value}." .

:UtilitySuperEffective a :Option ;
  rdfs:label "Super Effective" ;
  rdfs:comment "Yes to automatable and concentrated value." .

:Automatable a :DecisionPoint ;
  rdfs:label "Automatable" ;
  rdfs:comment "A decision point representing whether an attacker can reliably automate creating exploitation events for a given vulnerability, including reconnaissance, weaponization, delivery, and exploitation steps in the kill chain." ;
  :hasOption :AutomatableNo, :AutomatableYes .

:AutomatableNo a :Option ;
  rdfs:label "No" ;
  rdfs:comment "Attackers cannot reliably automate steps 1-4 of the kill chain for this vulnerability." .

:AutomatableYes a :Option ;
  rdfs:label "Yes" ;
  rdfs:comment "Attackers can reliably automate steps 1-4 of the kill chain for this vulnerability." .

